src/tls/TLSInfo.fst
@@ -88,10 +88,10 @@ request_client_certificate: single_assign ServerCertificateRequest // uses this 
 
 type config = {
     (* Supported versions, ciphersuites, and compressions *)
-    minVer: ProtocolVersion;
-    maxVer: ProtocolVersion;
+    minVer: protocolVersion;
+    maxVer: protocolVersion;
     ciphersuites: x:known_cipher_suites{List.Tot.length x < 256};
-    compressions: l:list Compression{ List.Tot.length l <= 1 };
+    compressions: l:list compression{ List.Tot.length l <= 1 };
 
     (* Handshake specific options *)
 
@@ -111,7 +111,7 @@ type config = {
 
     (* Sessions database *)
     sessionDBFileName: string;
-    sessionDBExpiry: TimeSpan;
+    sessionDBExpiry: timeSpan;
 
     (* DH groups database *)
     dhDBFileName: string;
@@ -169,14 +169,14 @@ let defaultConfig =
 type random = lbytes 32
 type crand = random
 type srand = random
-type CsRands = bytes
+type csRands = bytes
 
 type cVerifyData = bytes (* ClientFinished payload *)
 type sVerifyData = bytes (* ServerFinished payload *)
 
 type sessionHash = bytes
 
-let noCsr:CsRands = Nonce.noCsr
+let noCsr:csRands = Nonce.noCsr
 
 // -------------------------------------------------------------------
 // We support these extensions, with session scopes
@@ -268,11 +268,11 @@ let strongKEX = function
 // CF postv1, move strength predicates --> TLSConstants
 // ``kefAlg is a strong randomness extractor, despite all other kefAlgs'', guarding idealization in KEF
 
-assume val strongKEF: KefAlg -> Tot bool
+assume val strongKEF: kefAlg_t -> Tot bool
 
 // guarding idealizations for KDF and VerifyData (see PRF.fs)
-assume val strongKDF: KdfAlg -> Tot bool
-assume val strongVD: VdAlg -> Tot bool
+assume val strongKDF: kdfAlg_t -> Tot bool
+assume val strongVD: vdAlg_t -> Tot bool
 
 // -------------------------------------------------------------------
 // Session information (public immutable data)
@@ -281,12 +281,12 @@ type sessionID = b:bytes { length b <= 32 }
 // ``An arbitrary byte sequence chosen by the server
 // to identify an active or resumable session state.''
 
-type SessionInfo = {
+type sessionInfo = {
     init_crand: crand;
     init_srand: srand;
-    protocol_version: p:ProtocolVersion; // { p <> TLS_1p3 };
+    protocol_version: p:protocolVersion; // { p <> TLS_1p3 };
     cipher_suite: cipherSuite;
-    compression: Compression;
+    compression: compression;
     extensions: negotiatedExtensions;
     pmsId: pmsId;
     session_hash: sessionHash;
@@ -304,13 +304,13 @@ type SessionInfo = {
 // for certificates, the empty list represents the absence of identity
 // (possibly refusing to present requested certs)
 
-val csrands: SessionInfo -> Tot CsRands
+val csrands: sessionInfo -> Tot csRands
 let csrands si = si.init_crand @| si.init_srand
 //CF subsumes mk_csrands
 
-// Getting algorithms from SessionInfo
+// Getting algorithms from sessionInfo
 //CF subsume mk_kefAlg, mk_kefAlgExtended, mk_kdfAlg
-val kefAlg: si:SessionInfo { is_Some (prfMacAlg_of_ciphersuite_aux si.cipher_suite) } -> Tot KefAlg
+val kefAlg: si:sessionInfo { is_Some (prfMacAlg_of_ciphersuite_aux si.cipher_suite) } -> Tot kefAlg_t
 let kefAlg si =
   match si.protocol_version with
   | SSL_3p0           -> PRF_SSL3_nested
@@ -318,7 +318,7 @@ let kefAlg si =
   | TLS_1p2           -> PRF_TLS_1p2 extract_label (prfMacAlg_of_ciphersuite si.cipher_suite)
   | TLS_1p3           -> PRF_TLS_1p3 //TBC
 
-val kefAlgExtended: si:SessionInfo { is_Some (prfMacAlg_of_ciphersuite_aux si.cipher_suite) } -> Tot KefAlg
+val kefAlgExtended: si:sessionInfo { is_Some (prfMacAlg_of_ciphersuite_aux si.cipher_suite) } -> Tot kefAlg_t
 let kefAlgExtended si =
   match si.protocol_version with
   | SSL_3p0           -> PRF_SSL3_nested
@@ -326,7 +326,7 @@ let kefAlgExtended si =
   | TLS_1p2           -> PRF_TLS_1p2 extended_extract_label (prfMacAlg_of_ciphersuite si.cipher_suite)
   | TLS_1p3           -> PRF_TLS_1p3 //TBC
 
-val kdfAlg: si:SessionInfo { is_Some (prfMacAlg_of_ciphersuite_aux si.cipher_suite) } -> Tot KdfAlg
+val kdfAlg: si:sessionInfo { is_Some (prfMacAlg_of_ciphersuite_aux si.cipher_suite) } -> Tot kdfAlg_t
 let kdfAlg si =
   match si.protocol_version with
   | SSL_3p0           -> PRF_SSL3_nested
@@ -336,14 +336,14 @@ let kdfAlg si =
 
 let vdAlg si = si.protocol_version, si.cipher_suite
 
-val siAuthEncAlg: si:SessionInfo { si.protocol_version = TLS_1p2 &&
+val siAuthEncAlg: si:sessionInfo { si.protocol_version = TLS_1p2 &&
                               pvcs si.protocol_version si.cipher_suite } -> Tot aeAlg
 let siAuthEncAlg si = get_aeAlg si.cipher_suite
 
 type msId = // We record the parameters used to derive the master secret;
-  | StandardMS : pmsId -> CsRands -> KefAlg -> msId
+  | StandardMS : pmsId -> csRands -> kefAlg_t -> msId
             // the pms index, the nonces, and the PMS-PRF algorithm
-  | ExtendedMS : pmsId -> sessionHash -> KefAlg -> msId
+  | ExtendedMS : pmsId -> sessionHash -> kefAlg_t -> msId
             // the pms index, the hash of the session log, and the PMS-PRF algorithm
             // using the sessionHash instead of randoms prevent MiTM forwarding honest randoms
 
@@ -360,10 +360,10 @@ let honestMS = function
 val noMsId: i:msId { not (honestMS i) }
 let noMsId = StandardMS noPmsId noCsr PRF_SSL3_nested
 
-// Getting master-secret indexes out of SessionInfo
+// Getting master-secret indexes out of sessionInfo
 
 //CF subsumes both MsI and mk_msid
-val msid: si:SessionInfo { is_Some (prfMacAlg_of_ciphersuite_aux (si.cipher_suite)) } -> Tot msId
+val msid: si:sessionInfo { is_Some (prfMacAlg_of_ciphersuite_aux (si.cipher_suite)) } -> Tot msId
 let msid si =
   if si.extensions.ne_extended_ms
   then ExtendedMS si.pmsId si.session_hash (kefAlgExtended si)
@@ -389,7 +389,7 @@ let strongHS si =
   strongPRF si &&
   strongSig si  //CF * hashAlg for certs?
 
-// Safety of SessionInfo crypto processing
+// Safety of sessionInfo crypto processing
 
 // Safe handshake for PMS-based extraction
 let safeCRE si = honestMS (msid si)
@@ -402,7 +402,7 @@ let safeVD si = honestMS (msid si) && strongVD(vdAlg si)
 assume val int_cma: macAlg -> Tot bool
 let strongAuthSI si = true //TODO: fix
 
-assume val strongAESI: SessionInfo -> Tot bool
+assume val strongAESI: sessionInfo -> Tot bool
 
 // -------------------------------------------------------------------
 // Epoch descriptors (public immutable data)
@@ -415,11 +415,11 @@ type abbrInfo =
 
 type preEpoch =
     | InitEpoch of role
-    | FullEpoch : SessionInfo  -> preEpoch -> preEpoch
+    | FullEpoch : sessionInfo  -> preEpoch -> preEpoch
     | AbbrEpoch : ai:abbrInfo -> resumed:preEpoch -> pred:preEpoch -> preEpoch
 
 (* previously the last two cases were
-    | SuccEpoch of crand * srand * si:SessionInfo * pred:preEpoch
+    | SuccEpoch of crand * srand * si:sessionInfo * pred:preEpoch
  *)
 
 (* we enforce a well-formed invariant to ensure the functions below
@@ -452,7 +452,7 @@ let rec peer = function
   | FullEpoch si p   -> FullEpoch si (peer p)
   | AbbrEpoch ai r p -> AbbrEpoch ai (peer r) (peer p)
 
-val epochSI: succEpoch -> Tot SessionInfo
+val epochSI: succEpoch -> Tot sessionInfo
 let epochSI = function
   | FullEpoch si pe -> si
   | AbbrEpoch ai (FullEpoch si pe1) pe2 -> si
@@ -475,12 +475,12 @@ let epochCSRands e =
   let e' : succEpoch = unsafe_coerce e in //TODO: THIS FAILS CURRENTLY! FIXME
   epochCRand e' @| epochSRand e'
 
-type preConnectionInfo = {
+type pre_connectionInfo = {
     role: role;      // cached, could be retrieved from id_out
     id_rand: random; // our random
     id_in: epoch;
     id_out: epoch}
-type ConnectionInfo = preConnectionInfo
+type connectionInfo = pre_connectionInfo
 
 //$ inline
 let connectionRole ci = ci.role
@@ -513,11 +513,11 @@ let strongAE e = strongAESI (epochSI e)
 type id = {
   // indexes and algorithms of the session used in the key derivation
   msId   : msId;            // the index of the master secret used for key derivation
-  kdfAlg : KdfAlg;          // the KDF algorithm used for key derivation
-  pv     : ProtocolVersion; // should be part of aeAlg
+  kdfAlg : kdfAlg_t;          // the KDF algorithm used for key derivation
+  pv     : protocolVersion; // should be part of aeAlg
   aeAlg  : aeAlg;           // the authenticated-encryption algorithms
   // epoch-specific parameters
-  csrConn: CsRands;         // the client-server random of the connection
+  csrConn: csRands;         // the client-server random of the connection
   ext: negotiatedExtensions;// the extensions negotiated for the current session
   writer : role             // the role of the writer
   }
@@ -526,7 +526,7 @@ let swap (i:id) = { i with writer = dualRole i.writer }
 let peerId (i:id) = { i with writer = dualRole i.writer }
 //let peerId = swap // better name?
 
-val siId: si:SessionInfo{ is_Some (prfMacAlg_of_ciphersuite_aux (si.cipher_suite))
+val siId: si:sessionInfo{ is_Some (prfMacAlg_of_ciphersuite_aux (si.cipher_suite))
 			  /\ ((si.protocol_version = TLS_1p2) && (pvcs si.protocol_version si.cipher_suite))} -> role -> Tot id
 let siId si r =
   { msId    = msid si;
@@ -556,7 +556,7 @@ let encAlg_of_id i = encAlg_of_aeAlg i.pv i.aeAlg
 let kdfAlg_of_id (i:id) = i.kdfAlg
 
 // Pretty printing
-let sinfo_to_string (si:SessionInfo) = ""
+let sinfo_to_string (si:sessionInfo) = ""
 (*
 #if 1 //TODO: This should be verify
 #else
@@ -596,19 +596,19 @@ let cipher_repr n = lemma_repr_bytes_values n
 
 //$ could be turnd into stateful logs; see F7 assumptions we made about them
 
-assume logic type KeyCommit   : CsRands -> ProtocolVersion -> aeAlg -> negotiatedExtensions -> Type
-assume logic type KeyGenClient: CsRands -> ProtocolVersion -> aeAlg -> negotiatedExtensions -> Type
-assume logic type SentCCS     : role -> SessionInfo -> Type
-assume logic type SentCCSAbbr : role -> abbrInfo -> Type
+assume logic type keyCommit   : csRands -> protocolVersion -> aeAlg -> negotiatedExtensions -> Type
+assume logic type keyGenClient: csRands -> protocolVersion -> aeAlg -> negotiatedExtensions -> Type
+assume logic type sentCCS     : role -> sessionInfo -> Type
+assume logic type sentCCSAbbr : role -> abbrInfo -> Type
 
 // ``the honest participants of handshake with this csr use matching aeAlgs''
-type Match (i:id) =
-    KeyCommit i.csrConn i.pv i.aeAlg i.ext
-    /\ KeyGenClient i.csrConn i.pv i.aeAlg i.ext
+type matches_id (i:id) =
+    keyCommit i.csrConn i.pv i.aeAlg i.ext
+    /\ keyGenClient i.csrConn i.pv i.aeAlg i.ext
 
 //$ recode?
 // This index is safe for MS-based key derivation
-val safeKDF: i:id -> Tot (b:bool { b=true <==> ((honestMS i.msId && strongKDF i.kdfAlg) /\ Match i) })
+val safeKDF: i:id -> Tot (b:bool { b=true <==> ((honestMS i.msId && strongKDF i.kdfAlg) /\ matches_id i) })
 //defining this as true makes the context inconsitent!
 let safeKDF _ = unsafe_coerce true //TODO: THIS IS A PLACEHOLDER
 
@@ -616,7 +616,7 @@ let safeKDF _ = unsafe_coerce true //TODO: THIS IS A PLACEHOLDER
 // ask !i1,i2. i2 = Swap(i1) /\ not(SafeKDF(i1)) => not(SafeKDF(i2))
 
 // HonestMS(msi) conditions both idealizations in PRF.
-// ask !si:SessionInfo. not HonestMS(MsI(si)) => not SafeVD(si)
+// ask !si:sessionInfo. not HonestMS(MsI(si)) => not SafeVD(si)
 // ask !i:id. not HonestMS(i.msId) => not SafeKDF(i)
 
 // -----------------------------------------------------------------------
@@ -631,7 +631,7 @@ let safeId (i:id) = safeKDF i && strongAEId i
 
 (* // ask !i.     SafeId(i) => AuthId(i) *)
 (* // ask !i,mac. i.aeAlg  = MACOnly(mac) => not SafeId(i) *)
-(* // ask !i:id. AuthId(i) => Match(i) // sanity check; just by definition *)
+(* // ask !i:id. AuthId(i) => matches_id(i) // sanity check; just by definition *)
 (* // ask !i:id. AuthId(i) => SafeKDF(i) *)
 (* // ask !i:id. AuthId(i) => StrongAuthId(i) *)
 (* // ask !i:id. AuthId(i) => INT_CMA_M(MacAlg(i)) *)
@@ -679,33 +679,39 @@ let mk_id e =
 // and performing both strong session key generation & finished message verification
 
 // Safe handshake for this sessioninfo
-type SafeHS_SI (si:SessionInfo) = ((is_Some (prfMacAlg_of_ciphersuite_aux (si.cipher_suite))) /\ (((si.protocol_version) = TLS_1p2) && (pvcs (si.protocol_version) (si.cipher_suite)))) /\ (honestPMS si.pmsId && strongHS si) /\ (exists r. Match(siId si r))
+let si_safeHS (si:sessionInfo) = 
+  is_Some (prfMacAlg_of_ciphersuite_aux si.cipher_suite) /\ 
+  si.protocol_version = TLS_1p2 /\
+  pvcs si.protocol_version si.cipher_suite /\ 
+  honestPMS si.pmsId /\
+  strongHS si /\ 
+  (exists r. matches_id (siId si r))
 
-// Safety for epochs relies only on SessionInfo.
+// Safety for epochs relies only on sessionInfo.
 // This would change if we introduced a finer model of compromise
 // e.g. if we allowed the attacker to compromise specific epochs
 
-type SafeHS (e:epoch) = is_SuccEpoch e /\ SafeHS_SI(epochSI e)
-assume val safeHS: e:epoch -> b:bool { b = true <==> SafeHS e }
+let epoch_safeHS (e:epoch) = is_SuccEpoch e /\ si_safeHS (epochSI e)
+assume val safeHS: e:epoch -> b:bool { b = true <==> epoch_safeHS e }
 
 // Predicates specifying the security of TLS connections
 
 // ``The handshake is complete''
-type Open (e:epoch) = ( exists (r:role).
-  (is_FullEpoch e /\ SentCCS r     (epochSI e) /\ SentCCS    (dualRole r) (epochSI e)) \/
-  (is_AbbrEpoch e /\ SentCCSAbbr r (epochAI e) /\ SentCCSAbbr(dualRole r) (epochAI e)))
+let epoch_open (e:epoch) = exists (r:role).
+  (is_FullEpoch e /\ sentCCS r     (epochSI e) /\ sentCCS    (dualRole r) (epochSI e)) \/
+  (is_AbbrEpoch e /\ sentCCSAbbr r (epochAI e) /\ sentCCSAbbr(dualRole r) (epochAI e))
 
-type OpenState (e:epoch) = ( exists (r:role).
-  (((is_FullEpoch e /\ is_Some (prfMacAlg_of_ciphersuite_aux (epochSI e).cipher_suite) /\  SentCCS r     (epochSI e) /\ safeVD (epochSI e)) ==> SentCCS    (dualRole r) (epochSI e))) \/
-  (((is_AbbrEpoch e /\ SentCCSAbbr r (epochAI e) /\ safeVD (epochSI e)) ==> SentCCSAbbr(dualRole r) (epochAI e))))
+let epoch_open_state (e:epoch) = exists (r:role).
+  (((is_FullEpoch e /\ is_Some (prfMacAlg_of_ciphersuite_aux (epochSI e).cipher_suite) /\  sentCCS r     (epochSI e) /\ safeVD (epochSI e)) ==> sentCCS    (dualRole r) (epochSI e))) \/
+  (((is_AbbrEpoch e /\ sentCCSAbbr r (epochAI e) /\ safeVD (epochSI e)) ==> sentCCSAbbr(dualRole r) (epochAI e)))
 
 // The epoch parameters yield privacy & integrity
-type Safe (e:epoch) =  (not (is_InitEpoch e)) ==> is_CipherSuite ((epochSI e).cipher_suite) /\ safeId (mk_id e) /\ OpenState e
-assume val safe: e:epoch -> b:bool { b = true <==> Safe e }
+let epoch_safe (e:epoch) =  (not (is_InitEpoch e)) ==> is_CipherSuite ((epochSI e).cipher_suite) /\ safeId (mk_id e) /\ epoch_open_state e
+assume val safe: e:epoch -> b:bool { b = true <==> epoch_safe e }
 
 // The epoch parameters yield integrity (not necessarily privacy)
-type Auth (e:epoch) = (not (is_InitEpoch e)) ==> is_CipherSuite ((epochSI e).cipher_suite) /\ ((is_MtE (mk_id e).aeAlg) \/ (is_MACOnly (mk_id e).aeAlg /\ is_SSL_3p0 ((mk_id e).pv))) /\ authId (mk_id e) /\ OpenState e
-assume val auth: e:epoch -> b:bool { b = true <==> Auth e }
+let epoch_auth (e:epoch) = (not (is_InitEpoch e)) ==> is_CipherSuite ((epochSI e).cipher_suite) /\ ((is_MtE (mk_id e).aeAlg) \/ (is_MACOnly (mk_id e).aeAlg /\ is_SSL_3p0 ((mk_id e).pv))) /\ authId (mk_id e) /\ epoch_open_state e
+assume val auth: e:epoch -> b:bool { b = true <==> epoch_auth e }
 
 //ask !e. Safe(e) => Auth(e)
 //ask !e. not(Auth(e)) => not(Safe(e))
@@ -713,30 +719,30 @@ assume val auth: e:epoch -> b:bool { b = true <==> Auth e }
 // so that TLS can exchange any traffic on the initial null connection
 //ask !e. IsInitEpoch(e) => not Auth(e)
 
-//ask !e. OpenState(e) => (AuthId(Id(e)) => Auth(e))
-//ask !e. OpenState(e) => (SafeId(Id(e)) => Safe(e))
-//ask !e. Auth(e) => OpenState(e)
+//ask !e. epoch_open_state(e) => (AuthId(Id(e)) => Auth(e))
+//ask !e. epoch_open_state(e) => (SafeId(Id(e)) => Safe(e))
+//ask !e. Auth(e) => epoch_open_state(e)
 
 
 (*
   KB The following is only true with Reneg indication, but is difficult to remove.
   KB It is an artifact of the way we treat epochs that we cannot just authenticate the current epoch, we need to always authenticate the full chain
   KB Maybe a refactor for v2 would be to separate our the current epoch and an optional predecessor
-  KB Also this needs to account for SentCCSResume
+  KB Also this needs to account for sentCCSResume
   
-private theorem !r,r',e,e'. SentCCS(r,EpochSI(e)) /\
-	                    SentCCS(r',EpochSI(e')) /\
+private theorem !r,r',e,e'. sentCCS(r,EpochSI(e)) /\
+	                    sentCCS(r',EpochSI(e')) /\
   			    Id(e) = Id(e') => e = e'
-theorem !e,e'. OpenState(e) /\ OpenState(e') /\ Id(e) = Id(e') => e = e'
+theorem !e,e'. epoch_open_state(e) /\ epoch_open_state(e') /\ Id(e) = Id(e') => e = e'
  *)
 
 (*
 #if ideal
 // These functions are used only for specifying ideal implementations
 let safeHS (e:epoch) = failwith "spec only": bool
-let safeHS_SI (e:SessionInfo) = failwith "spec only": bool
-let safeCRE (e:SessionInfo) = failwith "spec only": bool
-let safeVD (e:SessionInfo) = failwith "spec only": bool
+let safeHS_SI (e:sessionInfo) = failwith "spec only": bool
+let safeCRE (e:sessionInfo) = failwith "spec only": bool
+let safeVD (e:sessionInfo) = failwith "spec only": bool
 let auth (e:epoch) = failwith "spec only": bool
 let safe (e:epoch) = failwith "spec only" : bool //CF Define in terms of strength and honesty
 let safeKDF (i:id) = failwith "spec only": bool
