src/tls/Record.fst
@@ -48,7 +48,7 @@ assume val is_Null: id -> Tot bool
 // hopefully we only care about the writer, not the cn state
 // the postcondition is of the form
 //   authId i ==> f is added to the writer log
-let recordPacketOut (i: AEAD_GCM.gid) (wr:StatefulLHAE.writer i) (pv: ProtocolVersion) f =
+let recordPacketOut (i: AEAD_GCM.gid) (wr:StatefulLHAE.writer i) (pv: protocolVersion) f =
     let ct, rg = Content.ct_rg i f in
     let payload =
       if is_Null i
