src/tls/artifact/AEAD_GCM.fst
@@ -121,7 +121,7 @@ let leak i role s = State.key s @| State.iv s
 val enc:
   i:gid -> e:encryptor i -> ad:adata i
   -> r:range{fst r = snd r /\ snd r <= max_TLSPlaintext_fragment_length}
-  -> p:bytes{Within (length p) r}
+  -> p:bytes{within (length p) r}
   -> ST (cipher i)
     (requires (fun h -> True))
     (ensures  (fun h0 c h1 ->
